implicit arguments for iffH (to do:  existH, etc.)

theories/ordinals/Ackermann/LNN.v
@@ -17,7 +17,6 @@ Definition Term := Term LNN.
 Definition Terms := Terms LNN.
 Definition var := var LNN.
 Definition equal := equal LNN.
-Definition iffH := iffH LNN.
 Definition existH := existH LNN.
 Definition ifThenElseH := ifThenElseH LNN.
 Definition SysPrf := SysPrf LNN.
